more progress

dsl/src/dsl.ml
@@ -446,6 +446,10 @@ let toSZ e = Fn (ToSZ, [e])
 
 let toUZ e = Fn (ToUZ, [e])
 
+let q_ind' e q1 q2 = qand (qimply (qleq z1 (toUZ e)) q1) (qimply (qeq e f0) q2)
+
+let q_ind_dec' e q = q_ind' e q (qnot q)
+
 let f_range l r =
   TRef (tf, qand (lift (leq l (toUZ nu))) (lift (leq (toUZ nu) r)))
 
