dsl/src/typecheck.ml
@@ -373,7 +373,7 @@ let rec synthesize (e : expr) : typ S.t =
                 failwith "[synthesize] get: not an array" )
         | ArrayOp (Take, [e1; e2]) -> (
             let%bind t1 = synthesize e1 in
-            match skeleton t1 with
+            match descale t1 with
             | TArr te ->
                 let%bind () = check e2 tint in
                 return (tarr_t_q_k te (nu ==. e) e2)
@@ -381,7 +381,7 @@ let rec synthesize (e : expr) : typ S.t =
                 failwith "[synthesize] take: not an array" )
         | ArrayOp (Drop, [e1; e2]) -> (
             let%bind t1 = synthesize e1 in
-            match skeleton t1 with
+            match descale t1 with
             | TArr te ->
                 let%bind () = check e2 tint in
                 return (tarr_t_q_k te (nu ==. e) (len e1 -. e2))
